neaten up utils

Util.thy
@@ -173,8 +173,6 @@ definition \<open>prepost_state \<equiv> pre_state \<squnion> post_state\<close>
 
 lemmas prepost_state_def' = prepost_state_def pre_state_def post_state_def
 
-abbreviation \<open>quasireflp r \<equiv> reflp_on (Collect (prepost_state r)) r\<close>
-
 definition \<open>pre_change_state r \<equiv> \<lambda>a. \<exists>b. r a b \<and> a \<noteq> b\<close>
 definition \<open>post_change_state r \<equiv> \<lambda>b. \<exists>a. r a b \<and> a \<noteq> b\<close>
 definition \<open>change_state \<equiv> pre_change_state \<squnion> post_change_state\<close>
@@ -216,6 +214,8 @@ lemma post_state_reldisj[simp]:
 
 
 subsubsection \<open> quasireflp \<close>
+
+abbreviation \<open>quasireflp r \<equiv> reflp_on (Collect (prepost_state r)) r\<close>
 
 lemma quasireflpD1[dest]:
   \<open>quasireflp r \<Longrightarrow> r x y \<Longrightarrow> r x x\<close>
@@ -861,35 +861,29 @@ end
 context boolean_algebra
 begin
 
-definition implies :: "'a \<Rightarrow> 'a \<Rightarrow> 'a" (infixr "\<leadsto>" 60) where
+definition impl :: "'a \<Rightarrow> 'a \<Rightarrow> 'a" (infixr "\<leadsto>" 60) where
   "a \<leadsto> b \<equiv> -a \<squnion> b"
 
-lemma implies_shunt:
+lemma impl_shunt:
   \<open>c \<sqinter> a \<le> b \<longleftrightarrow> c \<le> a \<leadsto> b\<close>
-  by (simp add: implies_def shunt1)
+  by (simp add: impl_def shunt1)
 
-lemma implies_shunt2:
+lemma impl_shunt2:
   \<open>-(a \<leadsto> b) \<le> c \<longleftrightarrow> a \<le> b \<squnion> c\<close>
-  by (simp add: implies_def shunt2)
+  by (simp add: impl_def shunt2)
 
-lemma implies_simps[simp]:
-  \<open>(a \<leadsto> b) x = (a x \<longrightarrow> b x)\<close>
-  \<open>All (a \<leadsto> b) = (\<forall>x. a x \<longrightarrow> b x)\<close>
-  \<open>Ex (a \<leadsto> b) = (\<exists>x. a x \<longrightarrow> b x)\<close>
+lemma impl_simps[simp]:
   \<open>\<top> \<leadsto> b = b\<close>
   \<open>\<bottom> \<leadsto> b = \<top>\<close>
   \<open>a \<leadsto> \<bottom> = - a\<close>
   \<open>a \<leadsto> \<top> = \<top>\<close>
   \<open>a \<leadsto> a = \<top>\<close>
-  by (force simp add: boolean_algebra_class.implies_def)+
+  by (force simp add: impl_def)+
 
 definition bequiv :: "'a \<Rightarrow> 'a \<Rightarrow> 'a" (infixr "\<sim>" 60) where
   "a \<sim> b \<equiv> (a \<leadsto> b) \<sqinter> (b \<leadsto> a)"
 
 lemma bequiv_simps[simp]:
-  \<open>(a \<sim> b) x = (a x = b x)\<close>
-  \<open>All (a \<sim> b) = (\<forall>x. a x = b x)\<close>
-  \<open>Ex (a \<sim> b) = (\<exists>x. a x = b x)\<close>
   \<open>a \<sim> a = \<top>\<close>
   \<open>a \<sim> -a = \<bottom>\<close>
   \<open>-a \<sim> a = \<bottom>\<close>
@@ -897,19 +891,40 @@ lemma bequiv_simps[simp]:
   \<open>\<top> \<sim> a = a\<close>
   \<open>a \<sim> \<bottom> = -a\<close>
   \<open>\<bottom> \<sim> a = -a\<close>
-  by (force simp add: boolean_algebra_class.bequiv_def)+
+  by (clarsimp simp add: bequiv_def impl_def)+
 
 lemma bequiv_iff: \<open>a \<sim> b = (-a \<squnion> b) \<sqinter> (-b \<squnion> a)\<close>
-  by (simp add: bequiv_def implies_def)
+  by (simp add: bequiv_def impl_def)
 
 lemma bequiv_iff2: \<open>a \<sim> b = (a \<sqinter> b) \<squnion> (-a \<sqinter> -b)\<close>
   using bequiv_iff sup.commute sup_inf_distrib2 by force
 
 end
 
-lemma mem_implies_iff[simp]:
+lemma mem_impl_iff[simp]:
   \<open>x \<in> A \<leadsto> B \<longleftrightarrow> (x \<in> A \<longrightarrow> x \<in> B)\<close>
-  by (simp add: implies_def)
+  by (simp add: impl_def)
+
+lemma pred_impl_apply[simp]:
+  \<open>(a \<leadsto> b) x = (a x \<longrightarrow> b x)\<close>
+  by (simp add: impl_def)
+
+lemma rel_impl_apply[simp]:
+  \<open>(a \<leadsto> b) x y = (a x y \<longrightarrow> b x y)\<close>
+  by (simp add: impl_def)
+
+lemma mem_bequiv_iff[simp]:
+  \<open>x \<in> A \<sim> B \<longleftrightarrow> (x \<in> A \<longleftrightarrow> x \<in> B)\<close>
+  by (force simp add: bequiv_def)
+
+lemma pred_bequiv_apply[simp]:
+  \<open>(a \<sim> b) x \<longleftrightarrow> (a x = b x)\<close>
+  by (force simp add: bequiv_def)
+
+lemma rel_bequiv_apply[simp]:
+  \<open>(a \<sim> b) x y = (a x y = b x y)\<close>
+  by (force simp add: bequiv_def)
+
 
 subsection \<open> Bounded distributive lattices \<close>
 
